make the inhale and exhale relations with invariants the default, clean up the inhale and exhale invariant definitions
these new relations can be used to justify optimizations that make use of known information on the assertions

ExhaleRel.thy
@@ -5,11 +5,12 @@ begin
 
 definition exhale_rel :: 
     "('a full_total_state \<Rightarrow> 'a full_total_state \<Rightarrow> 'b nstate \<Rightarrow> bool)
+     \<Rightarrow> (assertion \<Rightarrow> 'a full_total_state \<Rightarrow> 'a full_total_state \<Rightarrow> bool)
      \<Rightarrow> 'a total_context
         \<Rightarrow> ('a full_total_state \<Rightarrow> bool)
-           \<Rightarrow> bigblock list \<Rightarrow> 'b econtext_bpl_general \<Rightarrow> (pure_exp, pure_exp atomic_assert) assert \<Rightarrow> bigblock \<times> cont \<Rightarrow> bigblock \<times> cont \<Rightarrow> bool"
-  where "exhale_rel R ctxt_vpr StateCons P ctxt assertion_vpr \<gamma> \<gamma>' \<equiv>
-         rel_general (uncurry R) (uncurry R)
+           \<Rightarrow> bigblock list \<Rightarrow> 'b econtext_bpl_general \<Rightarrow> assertion \<Rightarrow> bigblock \<times> cont \<Rightarrow> bigblock \<times> cont \<Rightarrow> bool"
+  where "exhale_rel R Q ctxt_vpr StateCons P ctxt assertion_vpr \<gamma> \<gamma>' \<equiv>
+         rel_general (uncurry (\<lambda>\<omega>def \<omega> ns. R \<omega>def \<omega> ns \<and> Q assertion_vpr \<omega>def \<omega>)) (uncurry R)
            \<comment>\<open>The well-definedness state remains the same\<close>
            (\<lambda> \<omega>0_\<omega> \<omega>0_\<omega>'. (fst \<omega>0_\<omega>) = (fst \<omega>0_\<omega>') \<and> red_exhale ctxt_vpr StateCons (fst \<omega>0_\<omega>) assertion_vpr (snd \<omega>0_\<omega>) (RNormal (snd \<omega>0_\<omega>')))
            (\<lambda> \<omega>0_\<omega>. red_exhale ctxt_vpr StateCons (fst \<omega>0_\<omega>) assertion_vpr (snd \<omega>0_\<omega>) RFailure)
@@ -22,7 +23,7 @@ lemma exhale_rel_intro:
           "\<And> \<omega>0 \<omega> ns. R \<omega>0 \<omega> ns \<Longrightarrow>
                       red_exhale ctxt_vpr StateCons \<omega>0 assertion_vpr \<omega> RFailure \<Longrightarrow>
                       \<exists>\<gamma>'. red_ast_bpl P ctxt (\<gamma>, Normal ns) (\<gamma>', Failure)"
-  shows "exhale_rel R ctxt_vpr StateCons P ctxt assertion_vpr \<gamma> \<gamma>'"
+  shows "exhale_rel R Q ctxt_vpr StateCons P ctxt assertion_vpr \<gamma> \<gamma>'"
   using assms
   using assms
   unfolding exhale_rel_def
@@ -32,85 +33,80 @@ lemma exhale_rel_intro_2:
   assumes
     "\<And>\<omega>0 \<omega> ns res. 
       R \<omega>0 \<omega> ns \<Longrightarrow> 
+      Q assertion_vpr \<omega>0 \<omega> \<Longrightarrow>
       red_exhale ctxt_vpr StateCons \<omega>0 assertion_vpr \<omega> res \<Longrightarrow>
       rel_vpr_aux (\<lambda>\<omega>' ns. R \<omega>0 \<omega>' ns) P ctxt \<gamma> \<gamma>' ns res"
-  shows "exhale_rel R ctxt_vpr StateCons P ctxt assertion_vpr \<gamma> \<gamma>'"
+  shows "exhale_rel R Q ctxt_vpr StateCons P ctxt assertion_vpr \<gamma> \<gamma>'"
   using assms
   unfolding exhale_rel_def rel_vpr_aux_def
   by (auto intro: rel_intro)
 
 lemma exhale_rel_normal_elim:
-  assumes "exhale_rel R ctxt_vpr StateCons P ctxt assertion_vpr \<gamma> \<gamma>'" and
-          "R \<omega>0 \<omega> ns" and
-          "red_exhale ctxt_vpr StateCons \<omega>0 assertion_vpr \<omega> (RNormal \<omega>')"
+  assumes "exhale_rel R Q ctxt_vpr StateCons P ctxt assertion_vpr \<gamma> \<gamma>'" 
+      and "R \<omega>0 \<omega> ns"
+      and "Q assertion_vpr \<omega>0 \<omega>"
+      and "red_exhale ctxt_vpr StateCons \<omega>0 assertion_vpr \<omega> (RNormal \<omega>')"
   shows "\<exists>ns'. red_ast_bpl P ctxt (\<gamma>, Normal ns) (\<gamma>', Normal ns') \<and> R \<omega>0 \<omega>' ns'"
   using assms
   unfolding exhale_rel_def rel_general_def
   by simp
 
 lemma exhale_rel_failure_elim:
-  assumes "exhale_rel R ctxt_vpr StateCons P ctxt assertion_vpr \<gamma> \<gamma>'" and
-          "R \<omega>0 \<omega> ns" and
-          "red_exhale ctxt_vpr StateCons \<omega>0 assertion_vpr \<omega> RFailure"
+  assumes "exhale_rel R Q ctxt_vpr StateCons P ctxt assertion_vpr \<gamma> \<gamma>'"
+     and  "R \<omega>0 \<omega> ns"
+     and  "Q assertion_vpr \<omega>0 \<omega>"
+     and  "red_exhale ctxt_vpr StateCons \<omega>0 assertion_vpr \<omega> RFailure"
         shows "\<exists>\<gamma>'. red_ast_bpl P ctxt (\<gamma>, Normal ns) (\<gamma>', Failure)"  
   using assms
   unfolding exhale_rel_def rel_general_def
   by simp
 
-subsection \<open>Exhale rel definition that can handle optimizations\<close>
+subsection \<open>Exhale relation invariant\<close>
 
-definition exhale_opt_rel :: 
-    "('a full_total_state \<Rightarrow> 'a full_total_state \<Rightarrow> 'b nstate \<Rightarrow> bool)
-     \<Rightarrow> ((pure_exp, pure_exp atomic_assert) assert \<Rightarrow> 'a full_total_state \<Rightarrow> 'a full_total_state \<Rightarrow> bool)
-     \<Rightarrow> 'a total_context
-        \<Rightarrow> ('a full_total_state \<Rightarrow> bool)
-           \<Rightarrow> bigblock list \<Rightarrow> 'b econtext_bpl_general \<Rightarrow> (pure_exp, pure_exp atomic_assert) assert \<Rightarrow> bigblock \<times> cont \<Rightarrow> bigblock \<times> cont \<Rightarrow> bool"
-  where "exhale_opt_rel R Q ctxt_vpr StateCons P ctxt assertion_vpr \<gamma> \<gamma>' \<equiv>
-         rel_general (uncurry (\<lambda>\<omega>def \<omega> ns. R \<omega>def \<omega> ns \<and> Q assertion_vpr \<omega>def \<omega>)) (uncurry R)
-           \<comment>\<open>The well-definedness state remains the same\<close>
-           (\<lambda> \<omega>0_\<omega> \<omega>0_\<omega>'. (fst \<omega>0_\<omega>) = (fst \<omega>0_\<omega>') \<and> red_exhale ctxt_vpr StateCons (fst \<omega>0_\<omega>) assertion_vpr (snd \<omega>0_\<omega>) (RNormal (snd \<omega>0_\<omega>')))
-           (\<lambda> \<omega>0_\<omega>. red_exhale ctxt_vpr StateCons (fst \<omega>0_\<omega>) assertion_vpr (snd \<omega>0_\<omega>) RFailure)
-           P ctxt \<gamma> \<gamma>'"
-
-definition is_assertion_red_invariant_2
-  where "is_assertion_red_invariant_2 ctxt StateCons Q Success \<equiv>
+definition is_exh_rel_invariant
+  where "is_exh_rel_invariant ctxt StateCons cond_assert cond_exp Q  \<equiv>
           \<comment>\<open>currently, just added no permission introspection, since it is required for framedness
              maybe should generalize to a parameter\<close>
-          (\<forall> A1 A2 \<omega>def \<omega>. Q (A1 && A2) \<omega>def \<omega> \<longrightarrow>
-                  no_perm_assertion A1 \<and> no_unfolding_assertion A1 \<longrightarrow> 
-                  (Q A1 \<omega>def \<omega>) \<and>
-                  (\<forall>\<omega>'. Success A1 \<omega>def \<omega> \<omega>' \<longrightarrow> Q A2 \<omega>def \<omega>')) \<and>
-          (\<forall> e A \<omega>def \<omega>. Q (assert.Imp e A) \<omega>def \<omega> \<longrightarrow> no_perm_pure_exp e \<and> no_unfolding_pure_exp e \<longrightarrow>
+          (\<forall> A1 A2 \<omega>def \<omega>. Q (A1 && A2) \<omega>def \<omega> \<and> cond_assert A1 \<longrightarrow>
+                  (Q A1 \<omega>def \<omega>) \<and> 
+                  (\<forall>\<omega>'. red_exhale ctxt StateCons \<omega>def A1 \<omega> (RNormal \<omega>') \<longrightarrow> Q A2 \<omega>def \<omega>')) \<and>
+          (\<forall> e A \<omega>def \<omega>. Q (assert.Imp e A) \<omega>def \<omega> \<and> cond_exp e \<longrightarrow>
                          ctxt, StateCons, Some \<omega>def \<turnstile> \<langle>e; \<omega>\<rangle> [\<Down>]\<^sub>t (Val (VBool True)) \<longrightarrow> Q A \<omega>def \<omega>)"
 
-lemma is_assertion_red_invariant_intro:
-  assumes "\<And> A1 A2 \<omega>def \<omega>. Q (A1 && A2) \<omega>def \<omega> \<Longrightarrow> no_perm_assertion A1 \<and> no_unfolding_assertion A1 \<Longrightarrow> Q A1 \<omega>def \<omega>" and
-          "\<And> A1 A2 \<omega>def \<omega> \<omega>'. Q (A1 && A2) \<omega>def \<omega> \<Longrightarrow> no_perm_assertion A1 \<and> no_unfolding_assertion A1 \<Longrightarrow> Success A1 \<omega>def \<omega> \<omega>' \<Longrightarrow> Q A2 \<omega>def \<omega>'" and
-          "\<And> e A \<omega>def \<omega>. Q (assert.Imp e A) \<omega>def \<omega> \<Longrightarrow> 
-                         no_perm_pure_exp e \<and> no_unfolding_pure_exp e \<Longrightarrow>
+lemma is_exh_rel_invariant_intro:
+  assumes "\<And> A1 A2 \<omega>def \<omega>. Q (A1 && A2) \<omega>def \<omega> \<Longrightarrow> cond_assert A1 \<Longrightarrow> Q A1 \<omega>def \<omega>" and
+          "\<And> A1 A2 \<omega>def \<omega> \<omega>'. Q (A1 && A2) \<omega>def \<omega>  \<Longrightarrow> cond_assert A1
+                                                    \<Longrightarrow> red_exhale ctxt StateCons \<omega>def A1 \<omega> (RNormal \<omega>') 
+                                                   \<Longrightarrow> Q A2 \<omega>def \<omega>'" and
+          "\<And> e A \<omega>def \<omega>. Q (assert.Imp e A) \<omega>def \<omega> \<Longrightarrow> cond_exp e \<Longrightarrow> 
                     ctxt, StateCons, Some \<omega>def \<turnstile> \<langle>e; \<omega>\<rangle> [\<Down>]\<^sub>t (Val (VBool True)) \<Longrightarrow> Q A \<omega>def \<omega>"
-        shows "is_assertion_red_invariant_2 ctxt StateCons Q Success"
+        shows "is_exh_rel_invariant ctxt StateCons cond_assert cond_exp Q"
   using assms
-  unfolding is_assertion_red_invariant_2_def
+  unfolding is_exh_rel_invariant_def
   by blast
 
-definition is_assertion_red_invariant_exh
-  where "is_assertion_red_invariant_exh ctxt_vpr StateCons Q \<equiv> 
-          is_assertion_red_invariant_2 ctxt_vpr StateCons Q (\<lambda>A \<omega>def \<omega> \<omega>'. red_exhale ctxt_vpr StateCons \<omega>def A \<omega> (RNormal \<omega>'))"
-
-subsubsection \<open>Invariant to be propagated for optimized exhale\<close> 
+subsubsection \<open>Invariant instantiations\<close> 
 
 definition framing_exh 
   where "framing_exh ctxt_vpr StateCons A \<omega>def \<omega> \<equiv>
            StateCons \<omega>def \<and> 
            valid_heap_mask (get_mh_total_full \<omega>def) \<and>
            (\<exists>\<omega>_inh \<omega>sum.  \<omega>_inh \<oplus> \<omega> = Some \<omega>sum \<and> \<omega>def \<succeq> \<omega>sum \<and> assertion_framing_state ctxt_vpr StateCons A \<omega>_inh)"  
+
+text \<open>\<^const>\<open>framing_exh\<close> expresses an exhale relation invariant from which one can show that the assertion is 
+      framed in the well-definedness state (due to monotonicity of framedness). 
+      \<^term>\<open>\<omega>_inh\<close> expresses the permissions that have been exhaled so far during the exhale. Since 
+      \<^const>\<open>framing_exh\<close> forces that \<^term>\<open>\<omega>_inh \<oplus> \<omega>\<close> does not exceed the well-definedness state, we know
+      that after exhaling a conjunct we can update \<^term>\<open>\<omega>_inh\<close> to a new normal state (instead of going to magic),
+      since we can exhale at most \<^term>\<open>\<omega>\<close>. This is required to prove that \<^const>\<open>framing_exh\<close> is an exhale
+      invariant.\<close>
         
 lemma framing_exh_is_assertion_red_invariant_exh:
   assumes MonoStateCons: "mono_prop_downward StateCons"
-  shows "is_assertion_red_invariant_exh ctxt_vpr StateCons (framing_exh ctxt_vpr StateCons)"
-  unfolding is_assertion_red_invariant_exh_def
-proof (rule is_assertion_red_invariant_intro)
+  shows "is_exh_rel_invariant ctxt_vpr StateCons (\<lambda>A. no_perm_assertion A \<and> no_unfolding_assertion A)
+                                                 (\<lambda>e. no_perm_pure_exp e \<and> no_unfolding_pure_exp e)
+                                                 (framing_exh ctxt_vpr StateCons)"
+proof (rule is_exh_rel_invariant_intro)
   \<comment>\<open>Separating Conjunction 1\<close>
   fix A1 A2 \<omega>def \<omega>
 
@@ -238,21 +234,22 @@ next
      by blast
 qed
     
- 
 subsection \<open>Propagation rules\<close>
 
 lemma exhale_rel_propagate_pre:
-  assumes "\<And> \<omega>0 \<omega> ns. R \<omega>0 \<omega> ns \<Longrightarrow> \<exists>ns'. red_ast_bpl P ctxt (\<gamma>0, Normal ns) (\<gamma>1, Normal ns') \<and> R \<omega>0 \<omega> ns'" and
-          "exhale_rel R ctxt_vpr StateCons P ctxt assertion_vpr \<gamma>1 \<gamma>2"
-        shows "exhale_rel R ctxt_vpr StateCons P ctxt assertion_vpr \<gamma>0 \<gamma>2"
-  using assms rel_propagate_pre
+  assumes PropagateBpl: "\<And> \<omega>0 \<omega> ns. R \<omega>0 \<omega> ns \<Longrightarrow> Q assertion_vpr \<omega>0 \<omega> \<Longrightarrow>
+           \<exists>ns'. red_ast_bpl P ctxt (\<gamma>0, Normal ns) (\<gamma>1, Normal ns') \<and> R \<omega>0 \<omega> ns'" 
+      and ExhRel: "exhale_rel R Q ctxt_vpr StateCons P ctxt assertion_vpr \<gamma>1 \<gamma>2"
+    shows "exhale_rel R Q ctxt_vpr StateCons P ctxt assertion_vpr \<gamma>0 \<gamma>2"
   unfolding exhale_rel_def
-  by (auto intro: rel_propagate_pre assms(1))
+  apply (rule rel_propagate_pre[OF _ ExhRel[simplified exhale_rel_def]])
+  by (auto intro: PropagateBpl)
 
 lemma exhale_rel_propagate_post:
-  assumes "exhale_rel R ctxt_vpr StateCons P ctxt assertion_vpr \<gamma>0 \<gamma>1" and
-          "\<And> \<omega>0 \<omega> ns. R \<omega>0 \<omega> ns \<Longrightarrow> \<exists>ns'. red_ast_bpl P ctxt (\<gamma>1, Normal ns) (\<gamma>2, Normal ns') \<and> R \<omega>0 \<omega> ns'"
-  shows "exhale_rel R ctxt_vpr StateCons P ctxt assertion_vpr \<gamma>0 \<gamma>2"
+  assumes "exhale_rel R Q ctxt_vpr StateCons P ctxt assertion_vpr \<gamma>0 \<gamma>1" and
+          "\<And> \<omega>0 \<omega> ns. R \<omega>0 \<omega> ns \<Longrightarrow> \<comment>\<open>Note that do not get Q in the post state for free\<close>
+                \<exists>ns'. red_ast_bpl P ctxt (\<gamma>1, Normal ns) (\<gamma>2, Normal ns') \<and> R \<omega>0 \<omega> ns'"
+  shows "exhale_rel R Q ctxt_vpr StateCons P ctxt assertion_vpr \<gamma>0 \<gamma>2"
   using assms
   unfolding exhale_rel_def
   by (auto intro: rel_propagate_post)
@@ -260,118 +257,51 @@ lemma exhale_rel_propagate_post:
 subsection \<open>Structural rules\<close>
 
 lemma exhale_rel_star: 
-  assumes "exhale_rel R ctxt_vpr StateCons P ctxt A1 \<gamma>1 \<gamma>2" and
-          "exhale_rel R ctxt_vpr StateCons P ctxt A2 \<gamma>2 \<gamma>3"
-        shows "exhale_rel R ctxt_vpr StateCons P ctxt (A1 && A2) \<gamma>1 \<gamma>3"
-  using assms
-  unfolding exhale_rel_def
-  apply (rule rel_general_comp)
-  by (fastforce elim: ExhStar_case)+
-
-lemma exhale_opt_rel_star: 
-  assumes Invariant1: "\<And> \<omega>def \<omega>. Q (A1 && A2) \<omega>def \<omega> \<Longrightarrow> Q A1 \<omega>def \<omega>" and
-          Invariant2: "\<And> \<omega>def \<omega> \<omega>'. Q (A1 && A2) \<omega>def \<omega> \<Longrightarrow> 
-                                    red_exhale ctxt_vpr StateCons \<omega>def A1 \<omega> (RNormal \<omega>') \<Longrightarrow> Q A2 \<omega>def \<omega>'" and
-          RelA1: "exhale_opt_rel R Q ctxt_vpr StateCons P ctxt A1 \<gamma>1 \<gamma>2" and
-          RelA2: "exhale_opt_rel R Q ctxt_vpr StateCons P ctxt A2 \<gamma>2 \<gamma>3"
-        shows "exhale_opt_rel R Q ctxt_vpr StateCons P ctxt (A1 && A2) \<gamma>1 \<gamma>3"
+  assumes Invariant1: "\<And> \<omega>def \<omega>. Q (A1 && A2) \<omega>def \<omega> \<Longrightarrow> Q A1 \<omega>def \<omega>"
+      and Invariant2: "\<And> \<omega>def \<omega> \<omega>'. Q (A1 && A2) \<omega>def \<omega> \<Longrightarrow> 
+                                    red_exhale ctxt_vpr StateCons \<omega>def A1 \<omega> (RNormal \<omega>') \<Longrightarrow> Q A2 \<omega>def \<omega>'"
+      and ExhRelA1: "exhale_rel R Q ctxt_vpr StateCons P ctxt A1 \<gamma>1 \<gamma>2"
+      and ExhRelA2: "exhale_rel R Q ctxt_vpr StateCons P ctxt A2 \<gamma>2 \<gamma>3"
+    shows "exhale_rel R Q ctxt_vpr StateCons P ctxt (A1 && A2) \<gamma>1 \<gamma>3"
   text\<open>Idea of proof:
        \<^item> use general composition rule where the intermediate relation is chosen to be \<^term>\<open>\<lambda>\<omega>def \<omega> ns. R \<omega>def \<omega> ns \<and> Q A2 \<omega>def \<omega>\<close>
        \<^item> Prove the first premise by weakening the input relation from \<^term>\<open>\<lambda>\<omega>def \<omega> ns. R \<omega>def \<omega> ns \<and> Q (A1 && A2) \<omega>def \<omega>\<close> 
          to \<^term>\<open>\<lambda>\<omega>def \<omega> ns. R \<omega>def \<omega> ns \<and> Q A1 \<omega>def \<omega>\<close> and by adjusting the output relation
          \<^term>\<open>\<lambda>\<omega>def \<omega> ns. R \<omega>def \<omega> ns \<and> Q A2 \<omega>def \<omega>\<close> to \<^term>\<open>R\<close> 
        (\<^term>\<open>R\<close> is strong enough given the additional assumptions when adjusting the output relation)\<close>
-  unfolding exhale_opt_rel_def
+  unfolding exhale_rel_def
   apply (rule rel_general_comp[where ?R2.0="uncurry (\<lambda>\<omega>def \<omega> ns. R \<omega>def \<omega> ns \<and> Q A2 \<omega>def \<omega>)"])
      apply (rule rel_general_conseq_input_output)
-       apply (rule RelA1[simplified exhale_opt_rel_def])
+       apply (rule ExhRelA1[simplified exhale_rel_def])
       apply (simp add: Invariant1)
      apply (fastforce dest: Invariant2)
-    apply (rule RelA2[simplified exhale_opt_rel_def])
+    apply (rule ExhRelA2[simplified exhale_rel_def])
   by (fastforce elim: ExhStar_case)+
 
+lemma exhale_rel_star_2: 
+  assumes Invariant: "is_exh_rel_invariant ctxt_vpr StateCons cond_assert cond_exp Q"
+      and Cond: "cond_assert A1"
+      and ExhRelA1: "exhale_rel R Q ctxt_vpr StateCons P ctxt A1 \<gamma>1 \<gamma>2"
+      and ExhRelA2: "exhale_rel R Q ctxt_vpr StateCons P ctxt A2 \<gamma>2 \<gamma>3"
+    shows "exhale_rel R Q ctxt_vpr StateCons P ctxt (A1 && A2) \<gamma>1 \<gamma>3"
+  apply (rule exhale_rel_star[OF _ _ ExhRelA1 ExhRelA2])
+  using Invariant Cond
+  unfolding is_exh_rel_invariant_def
+  by blast+
+
 lemma exhale_rel_imp:
-  assumes 
-   ExpWfRel:          
-        "expr_wf_rel R ctxt_vpr StateCons P ctxt cond 
-         \<gamma>1
-         (if_bigblock name (Some (cond_bpl)) (thn_hd # thn_tl) [empty_else_block], KSeq next cont)" 
-        (is "expr_wf_rel _ ctxt_vpr StateCons P ctxt cond _ ?\<gamma>_if") and
-   EmptyElse: "is_empty_bigblock empty_else_block" and
-   ExpRel: "exp_rel_vpr_bpl R ctxt_vpr ctxt cond cond_bpl" and
-   RhsRel: "exhale_rel R ctxt_vpr StateCons P ctxt A (thn_hd, convert_list_to_cont thn_tl (KSeq next cont)) (next, cont)"
-                (is "exhale_rel R _ _ _ _ _ ?\<gamma>_thn (next, cont)") 
-              shows "exhale_rel R ctxt_vpr StateCons P ctxt (assert.Imp cond A) \<gamma>1 (next, cont)"
-  unfolding exhale_rel_def 
-proof (simp only: uncurry.simps, rule rel_general_cond[OF rev_iffD1_def[OF wf_rel_inst_eq_1[OF ExpWfRel] wf_rel_inst_def]])
-  show "rel_general (\<lambda>\<omega>0_\<omega>. R (fst \<omega>0_\<omega>) (snd \<omega>0_\<omega>)) (\<lambda>\<omega>0_\<omega>. R (fst \<omega>0_\<omega>) (snd \<omega>0_\<omega>)) (\<lambda> \<omega> \<omega>'. \<omega> = \<omega>') (\<lambda>_. False) P ctxt (empty_else_block, convert_list_to_cont [] (KSeq next cont)) (next, cont)"
-    apply (rule rel_intro)
-    using red_ast_bpl_empty_block_2[OF EmptyElse]
-    apply fastforce
-    by simp
-next
-  let ?Success = "\<lambda>\<omega> \<omega>'. fst \<omega> = fst \<omega>' \<and> red_exhale ctxt_vpr StateCons (fst \<omega>) (assert.Imp cond A) (snd \<omega>) (RNormal (snd \<omega>'))"
-  let ?SuccessExp = "\<lambda>\<omega> \<omega>'. \<omega> = \<omega>' \<and> (\<exists>v. ctxt_vpr, StateCons, Some (fst \<omega>) \<turnstile> \<langle>cond;snd \<omega>\<rangle> [\<Down>]\<^sub>t Val v)"
-  let ?SuccessThn = "\<lambda>\<omega> \<omega>'. fst \<omega> = fst \<omega>' \<and> red_exhale ctxt_vpr StateCons (fst \<omega>) A (snd \<omega>) (RNormal (snd \<omega>'))"
-  let ?Fail ="\<lambda>\<omega>. red_exhale ctxt_vpr StateCons (fst \<omega>) (assert.Imp cond A) (snd \<omega>) RFailure"
-  let ?FailThn = "\<lambda>\<omega>. red_exhale ctxt_vpr StateCons (fst \<omega>) A (snd \<omega>) RFailure"
-  let ?FailExp = "\<lambda>\<omega>. ctxt_vpr, StateCons, Some (fst \<omega>) \<turnstile> \<langle>cond;snd \<omega>\<rangle> [\<Down>]\<^sub>t VFailure"
-
-  show "rel_general (\<lambda>a. R (fst a) (snd a)) (\<lambda>a. R (fst a) (snd a)) ?SuccessThn ?FailThn P ctxt (thn_hd, convert_list_to_cont thn_tl (KSeq next cont)) (next, cont)"
-    using RhsRel
-    unfolding exhale_rel_def
-    by simp
-  
-  show "\<And> \<omega> \<omega>' ns. ?Success \<omega> \<omega>' \<Longrightarrow> R (fst \<omega>) (snd \<omega>) ns \<Longrightarrow>
-                        ?SuccessExp \<omega> \<omega> \<and> \<comment>\<open>implicit assumption that success of conditional does not lead to side effects\<close>
-                       ((red_expr_bpl ctxt cond_bpl ns (BoolV True) \<and> R (fst \<omega>) (snd \<omega>) ns \<and> ?SuccessThn \<omega> \<omega>') \<or> 
-                       (red_expr_bpl ctxt cond_bpl ns (BoolV False) \<and> R (fst \<omega>) (snd \<omega>) ns \<and> \<omega> = \<omega>'))"
-             (is "\<And> \<omega> \<omega>' ns. _ \<Longrightarrow> _ \<Longrightarrow> ?Goal \<omega> \<omega>' ns")
-  proof - 
-    fix \<omega> \<omega>' ns
-    assume Success:"?Success \<omega> \<omega>'" and R: "R (fst \<omega>) (snd \<omega>) ns"
-    from conjunct2[OF \<open>?Success \<omega> \<omega>'\<close>]
-    show "?Goal \<omega> \<omega>' ns"
-      apply cases
-       apply (rule conjI)
-      apply blast
-      using exp_rel_vpr_bpl_elim_2[OF ExpRel] Success
-      apply (metis R val_rel_vpr_bpl.simps(2))
-      using exp_rel_vpr_bpl_elim_2[OF ExpRel] Success
-      by (metis R prod_eqI val_rel_vpr_bpl.simps(2))
-  qed
-
- show "\<And> \<omega> ns. ?Fail \<omega> \<Longrightarrow> R (fst \<omega>) (snd \<omega>) ns \<Longrightarrow> 
-               ?FailExp \<omega> \<or>
-               (?SuccessExp \<omega> \<omega> \<and>
-                 ( (red_expr_bpl ctxt cond_bpl ns (BoolV True) \<and> R (fst \<omega>) (snd \<omega>) ns \<and> ?FailThn \<omega>) \<or> 
-                   (red_expr_bpl ctxt cond_bpl ns (BoolV False) \<and> R (fst \<omega>) (snd \<omega>) ns \<and> False) )
-               )" (is "\<And> \<omega> ns. _ \<Longrightarrow> _ \<Longrightarrow> ?Goal \<omega> ns")
- proof -
-   fix \<omega> ns
-   assume Fail: "?Fail \<omega>" and "R (fst \<omega>) (snd \<omega>) ns" 
-   thus "?Goal \<omega> ns"
-     apply cases
-     using exp_rel_vpr_bpl_elim_2[OF ExpRel] Fail
-      apply (metis val_rel_vpr_bpl.simps(2))
-     by fast
- qed
-qed
-
-lemma exhale_opt_rel_imp:
-  assumes
-   Invariant: "\<And>\<omega>def \<omega>. ctxt_vpr, StateCons, Some \<omega>def \<turnstile> \<langle>cond; \<omega>\<rangle> [\<Down>]\<^sub>t (Val (VBool True)) \<Longrightarrow> Q (assert.Imp cond A) \<omega>def \<omega> \<Longrightarrow> Q A \<omega>def \<omega>" and
-   ExpWfRel: 
-        "expr_wf_rel R ctxt_vpr StateCons P ctxt cond 
-         \<gamma>1
-         (if_bigblock name (Some (cond_bpl)) (thn_hd # thn_tl) [empty_else_block], KSeq next cont)" 
-        (is "expr_wf_rel _ ctxt_vpr StateCons P ctxt cond _ ?\<gamma>_if") and
-   EmptyElse: "is_empty_bigblock empty_else_block" and
-   ExpRel: "exp_rel_vpr_bpl R ctxt_vpr ctxt cond cond_bpl" and
-   RhsRel: "exhale_opt_rel R Q ctxt_vpr StateCons P ctxt A (thn_hd, convert_list_to_cont thn_tl (KSeq next cont)) (next, cont)"
-                (is "exhale_opt_rel R Q _ _ _ _ _ ?\<gamma>_thn (next, cont)") 
-              shows "exhale_opt_rel R Q ctxt_vpr StateCons P ctxt (assert.Imp cond A) \<gamma>1 (next, cont)"
-  unfolding exhale_opt_rel_def
+  assumes Invariant: "\<And>\<omega>def \<omega>. ctxt_vpr, StateCons, Some \<omega>def \<turnstile> \<langle>cond; \<omega>\<rangle> [\<Down>]\<^sub>t (Val (VBool True)) \<Longrightarrow> Q (assert.Imp cond A) \<omega>def \<omega> \<Longrightarrow> Q A \<omega>def \<omega>"
+      and ExpWfRel: 
+          "expr_wf_rel R ctxt_vpr StateCons P ctxt cond 
+           \<gamma>1
+           (if_bigblock name (Some (cond_bpl)) (thn_hd # thn_tl) [empty_else_block], KSeq next cont)" 
+          (is "expr_wf_rel _ ctxt_vpr StateCons P ctxt cond _ ?\<gamma>_if")
+      and EmptyElse: "is_empty_bigblock empty_else_block"
+      and ExpRel: "exp_rel_vpr_bpl R ctxt_vpr ctxt cond cond_bpl"
+      and RhsRel: "exhale_rel R Q ctxt_vpr StateCons P ctxt A (thn_hd, convert_list_to_cont thn_tl (KSeq next cont)) (next, cont)"
+                (is "exhale_rel R Q _ _ _ _ _ ?\<gamma>_thn (next, cont)") 
+    shows "exhale_rel R Q ctxt_vpr StateCons P ctxt (assert.Imp cond A) \<gamma>1 (next, cont)"
+  unfolding exhale_rel_def
 proof (simp only: uncurry.simps, 
        rule rel_general_cond, 
        fastforce intro: rel_general_conseq_input_output[OF rev_iffD1_def[OF wf_rel_inst_eq_1[OF ExpWfRel] wf_rel_inst_def]])
@@ -390,7 +320,7 @@ next
 
   show "rel_general (\<lambda>a ns. R (fst a) (snd a) ns \<and> Q A (fst a) (snd a)) (\<lambda>a. R (fst a) (snd a)) ?SuccessThn ?FailThn P ctxt (thn_hd, convert_list_to_cont thn_tl (KSeq next cont)) (next, cont)"
     using RhsRel
-    unfolding exhale_opt_rel_def
+    unfolding exhale_rel_def
     by simp
   
   show "\<And> \<omega> \<omega>' ns. ?Success \<omega> \<omega>' \<Longrightarrow> R (fst \<omega>) (snd \<omega>) ns \<and> Q (assert.Imp cond A) (fst \<omega>) (snd \<omega>) \<Longrightarrow>
@@ -428,6 +358,24 @@ next
      by fast
  qed
 qed
+
+lemma exhale_rel_imp_2:
+  assumes Invariant: "is_exh_rel_invariant ctxt_vpr StateCons cond_assert cond_exp Q"
+      and Cond: "cond_exp cond"
+      and ExpWfRel: 
+          "expr_wf_rel R ctxt_vpr StateCons P ctxt cond 
+           \<gamma>1
+           (if_bigblock name (Some (cond_bpl)) (thn_hd # thn_tl) [empty_else_block], KSeq next cont)" 
+          (is "expr_wf_rel _ ctxt_vpr StateCons P ctxt cond _ ?\<gamma>_if")
+      and EmptyElse: "is_empty_bigblock empty_else_block"
+      and ExpRel: "exp_rel_vpr_bpl R ctxt_vpr ctxt cond cond_bpl"
+      and RhsRel: "exhale_rel R Q ctxt_vpr StateCons P ctxt A (thn_hd, convert_list_to_cont thn_tl (KSeq next cont)) (next, cont)"
+                (is "exhale_rel R Q _ _ _ _ _ ?\<gamma>_thn (next, cont)") 
+    shows "exhale_rel R Q ctxt_vpr StateCons P ctxt (assert.Imp cond A) \<gamma>1 (next, cont)"
+  apply (rule exhale_rel_imp[OF _ ExpWfRel EmptyElse ExpRel RhsRel])
+  using Invariant Cond
+  unfolding is_exh_rel_invariant_def
+  by blast
 
 subsection \<open>Field access predicate rule\<close>
 
@@ -481,7 +429,7 @@ lemma exhale_field_acc_rel:
                       (\<lambda> \<omega>0_\<omega> \<omega>0_\<omega>'. fst \<omega>0_\<omega> = fst \<omega>0_\<omega>' \<and> exhale_acc_normal_premise ctxt_vpr StateCons e_rcv_vpr f e_p p r (fst \<omega>0_\<omega>) (snd \<omega>0_\<omega>) (snd \<omega>0_\<omega>'))
                       (\<lambda>_. False) 
                       P ctxt \<gamma>3 \<gamma>'"
-  shows "exhale_rel R ctxt_vpr StateCons P ctxt (Atomic (Acc e_rcv_vpr f (PureExp e_p))) \<gamma> \<gamma>'"
+  shows "exhale_rel R Q ctxt_vpr StateCons P ctxt (Atomic (Acc e_rcv_vpr f (PureExp e_p))) \<gamma> \<gamma>'"
 proof (rule exhale_rel_intro_2)
   fix \<omega>0 \<omega> ns res
   assume R0:"R \<omega>0 \<omega> ns" 
@@ -693,15 +641,5 @@ next
     using \<open>temp_perm \<notin> _\<close> state_rel_aux_pred_remove
     using map_add_upd_left map_le_def by fastforce
 qed (auto)
-
-lemma red_exp_val_sub_exp_assertion_framing_state:
-assumes "assertion_framing_state ctxt StateCons (Atomic A) \<omega>_inh" and
-        "ctxt, StateCons, Some \<omega>_def \<turnstile> \<langle>e;\<omega>\<rangle> [\<Down>]\<^sub>t Val v" and
-        "sub_expressions_atomic A = e#es" and
-        "get_store_total \<omega> = get_store_total \<omega>_inh \<and>
-         get_trace_total \<omega> = get_trace_total \<omega>_inh \<and>
-         get_h_total_full \<omega> = get_h_total_full \<omega>_inh"
-shows "ctxt, StateCons, Some \<omega> \<turnstile> \<langle>e;\<omega>\<rangle> [\<Down>]\<^sub>t Val v"
-  oops
 
 end
